progress on an automated tactic ... but need to revise the occurrence of frame_wp in a WP

examples/seplogic/SL.Examples.fst
@@ -111,7 +111,8 @@ let split_lem #a #b sa sb = ()
 private let get_to_the_next_frame () :Tac unit =
   ignore (repeat (fun () -> apply_lemma (`split_lem); smt ()))
 
-#reset-options "--using_facts_from '* -FStar.Tactics -FStar.Reflection' --use_two_phase_tc false --__temp_fast_implicits"
+// --using_facts_from '* -FStar.Tactics -FStar.Reflection' 
+#reset-options "--use_two_phase_tc false --__temp_fast_implicits"
 
 open PatternMatching
 open CanonCommMonoid
@@ -133,10 +134,11 @@ let solve_frame_wp_fails (_:unit) : Tac unit =
 let frame_wp_qn = ["SL" ; "Effect" ; "frame_wp"]
 let write_wp_qn = ["SL" ; "Effect" ; "write_wp"]
 let read_wp_qn = ["SL" ; "Effect" ; "read_wp"]
+let bind_wp_qn = ["SL" ; "Effect" ; "bind_wp"]
+let framepost_qn = ["SL" ; "Effect" ; "frame_post"]
 let pointsto_qn = ["SepLogic"; "Heap"; "op_Bar_Greater"]
 
 let footprint_of (t:term) : Tac (list term) =
-  admit();
   let hd, tl = collect_app t in
   match inspect hd, tl with
   | Tv_FVar fv, [(ta, Q_Implicit); (tr, Q_Explicit); (tv, Q_Explicit)] ->
@@ -164,7 +166,6 @@ let frame_wp_lemma_with_squashes (m m0 m1:memory) (a:Type) (wp:st_wp a)
          (squash (frame_wp wp f_post m)) = ()
 
 let pointsto_to_string (fp_refs:list term) (t:term) : Tac string =
-  admit();
   let hd, tl = collect_app t in
   // dump (term_to_string hd);
   match inspect hd, tl with
@@ -259,7 +260,7 @@ let solve_read () : Tac unit =
   //; dump "after solve_read"
 
 let foo (_:unit) : Tac unit =
-   admit();
+   dump "start";
    norm [delta_only [%`st_stronger; "Prims.auto_squash"]];
    mapply (`FStar.Squash.return_squash);
    let post = forall_intro () in
@@ -270,6 +271,7 @@ let foo (_:unit) : Tac unit =
      let hm0 = implies_intro() in
      rewrite hm0; clear hm0;
      let rest = implies_intro() in
+   dump "after prelude";     
    norm [delta_only [%`bind_wp]];
    dump "solve_wp";
    let fp, frame = solve_frame_wp() in
@@ -282,530 +284,694 @@ let foo (_:unit) : Tac unit =
    solve_read();
    smt() //definedness
 
+noeq
+type cmd =
+  | Frame : ta:term -> twp:term -> tpost:term -> tm:term -> cmd
+  | Read      : cmd
+  | Write     : cmd  
+  | Bind      : cmd
+  | FramePost : cmd
+  | Unknown : cmd
+  
+let peek_cmd () : Tac cmd =
+  let g = cur_goal () in
+  let hd, tl = collect_app g in
+  match inspect hd, tl with
+  | Tv_FVar fv, [(t1, Q_Explicit)] ->
+    if inspect_fv fv = squash_qn then
+      (* is the goal fram_wp *)
+      let hd, tl = collect_app t1 in
+      (match inspect hd with
+      | Tv_FVar fv  ->
+       if inspect_fv fv = frame_wp_qn 
+       then match tl with
+            | [(ta, Q_Implicit);
+               (twp, Q_Explicit);
+               (tpost, Q_Explicit);
+               (tm, Q_Explicit)] -> Frame ta twp tpost tm
+            | _ -> fail "Unexpected arity of frame"
+       else if inspect_fv fv = read_wp_qn 
+       then Read
+       else if inspect_fv fv = write_wp_qn 
+       then Write
+       else if inspect_fv fv = bind_wp_qn
+       then Bind
+       else if inspect_fv fv = framepost_qn
+       then FramePost
+       else Unknown
+      | _ -> Unknown)
+   else fail "Unrecognized command: not a squash"
+ | _ -> fail "Unrecognized command: not an fv app"
+
+let rewrite_bind_eq (r:range) (a:Type) (b:Type) (wp1:st_wp a) (wp2:a -> st_wp b) (post:post b) (m0:memory) (rhs:Type)
+  : Lemma (requires (frame_wp wp1 (frame_post (fun x m1 -> frame_wp (wp2 x) (frame_post post) m1)) m0 == rhs))
+          (ensures (bind_wp r a b wp1 wp2 post m0 == rhs))
+  = ()           
+
+let rewrite_frame_post (a:Type) (p:post a) (m0:memory) (x:a) (m1:memory) (rhs:Type)
+  : Lemma (requires ((defined (m1 <*> m0) /\ p x (m1 <*> m0)) == rhs))
+          (ensures (frame_post #a p m0 x m1 == rhs))
+  = ()           
+
+let rewrite_read_wp (a:Type) (r:ref a) (post:post a) (m0:memory) (rhs:Type)
+  : Lemma (requires ( (exists (x:a). m0 == (r |> x) /\ post x m0) == rhs))
+          (ensures (read_wp #a r post m0 == rhs))
+  = () //assert_norm (read_wp #a r == (fun post m0 -> exists (x:a). m0 == (r |> x) /\ post x m0))
+
+let rewrite_write_wp (a:Type) (r:ref a) (v:a) (post:post unit) (m0:memory) (rhs:Type)
+  : Lemma (requires ((exists (x:a). m0 == (r |> x) /\ post () (r |> v)) == rhs))
+          (ensures (write_wp #a r v post m0 == rhs))
+  = () //assert_norm (write_wp #a r v == (fun post m0 -> exists (x:a). m0 == (r |> x) /\ post () (r |> v)))
+  
+let unfold_first_occurrence (name:string) (lem:term) : Tac unit =
+  let should_rewrite (s:term) : Tac (bool * int) =
+    let hd, _ = collect_app s in
+    match inspect hd with
+    | Tv_FVar fv ->
+      if flatten_name (inspect_fv fv) = name 
+      then true, 2
+      else false, 0
+    | _ -> false, 0
+  in
+  let rewrite () : Tac unit =
+    mapply lem;
+    trefl()
+  in
+  topdown_rewrite should_rewrite rewrite
+
+let rec sl (i:int) : Tac unit =
+  dump ("SL :" ^ string_of_int i);
+//  admit();
+  match peek_cmd () with
+  | Unknown -> smt ()
+  
+  | Bind -> 
+    unfold_first_occurrence (%`bind_wp) (`rewrite_bind_eq);
+    norm[];
+    sl (i + 1)
+
+  | Read -> 
+    unfold_first_occurrence (%`read_wp) (`rewrite_read_wp);
+    norm[];
+    eexists unit (fun () -> FStar.Tactics.split(); trefl());
+    sl (i + 1)
+
+  | Write -> 
+    unfold_first_occurrence (%`write_wp) (`rewrite_write_wp);
+    norm[];
+    eexists unit (fun () -> FStar.Tactics.split(); trefl());   
+    sl (i + 1)
+
+  | FramePost -> 
+    unfold_first_occurrence (%`frame_post) (`rewrite_frame_post);
+    norm[];
+    FStar.Tactics.split(); smt(); //definedness
+    sl (i + 1)
+
+  | Frame ta twp tpost tm ->
+        let fp_refs = footprint_of twp in
+        // dump ("fp_refs="^ FStar.String.concat ","
+        //   (List.Tot.map term_to_string fp_refs));
+        let fp = FStar.Tactics.Derived.fold_left
+                   (fun a t -> if term_eq a (`emp) then t
+                               else mk_e_app (`( <*> )) [a;t])
+                   (`emp)
+                   (FStar.Tactics.Derived.map
+                     (fun t -> let u = fresh_uvar (Some (`int)) in
+                               mk_e_app (`( |> )) [t; u]) fp_refs) in
+        // dump ("m0=" ^ term_to_string fp);
+        let env = cur_env () in
+        let frame = uvar_env env (Some (`memory)) in
+        let tp : term = mk_app (`eq2)
+              [((`memory),                     Q_Implicit);
+               (mk_e_app (`(<*>)) [fp;frame],  Q_Explicit);
+               (tm,                            Q_Explicit)] in
+        let new_goal = mk_e_app (pack_fv' squash_qn) [tp] in
+        let heq = tcut new_goal in
+        // dump "with new goal:";
+        flip();
+        // dump ("before canon_monoid");
+        canon_monoid_sl fp_refs memory_cm;
+        // dump ("after canon_monoid");
+        trefl();
+        // dump ("after trefl");
+        // let fp : term = norm_term [] fp in
+        // let frame : term = norm_term [] frame in
+        // dump ("m0/fp=" ^ term_to_string fp ^ "\n" ^
+        //       "m1/frame=" ^ term_to_string frame ^ "\n" ^
+        //       "a/ta=" ^ term_to_string ta ^ "\n" ^
+        //       "wp/twp=" ^ term_to_string twp ^ "\n" ^
+        //       "f_post/tpost=" ^ term_to_string tpost);
+        apply_lemma (mk_e_app (`frame_wp_lemma_with_squashes)
+                       [tm; fp; frame; ta; twp; tpost; binder_to_term heq]);
+        FStar.Tactics.split(); smt(); //definedness
+        // dump ("after frame lemma");
+        sl(i + 1)
+
+let prelude' () : Tac unit =
+   dump "start";
+   norm [delta_only [%`st_stronger; "Prims.auto_squash"]];
+   mapply (`FStar.Squash.return_squash);
+   let post = forall_intro () in
+   let m0 = forall_intro () in
+   let wp_annot = implies_intro() in
+   and_elim (pack (Tv_Var (fst (inspect_binder wp_annot))));
+   clear wp_annot;
+   let hm0 = implies_intro() in
+   rewrite hm0; clear hm0;
+   ignore (implies_intro() )
+
+let sl' () : Tac unit =
+   prelude'();
+   dump "after prelude";
+   sl(0)
+
 (*
  * two commands
  *)
+//#set-options "--debug SL.Examples --debug_level TacVerbose"
 let write_read (r1 r2:ref int) (x y:int) =
   (r1 := 2;
    !r2)
   <: STATE int (fun p m -> m == ((r1 |> x) <*> (r2 |> y)) /\ (defined m /\ p y ((r1 |> 2) <*> (r2 |> y))))
-  by foo
+  by sl'
 
-//       // prelude ();
-//       // process_command ();
-//       // get_to_the_next_frame ();
-//       // apply_lemma (`lemma_rewrite_sep_comm);
-//       // process_command ())
+let read_write (r1 r2:ref int) (x y:int) =
+  (let x = !r1 in
+   r2 := x)
+  <: STATE unit (fun p m -> m == ((r1 |> x) <*> (r2 |> y)) /\ (defined m /\ p () ((r1 |> x) <*> (r2 |> x))))
+  by sl'
 
-// (*
-//  * four commands
-//  *)
-// let swap (r1 r2:ref int) (x y:int)
-//   = (let x = !r1 in
-//      let y = !r2 in
-//      r1 := y;
-//      r2 := x)
+(*
+// //  * four commands
+// //  *)
+let swap (r1 r2:ref int) (x y:int)
+  = (let x = !r1 in
+     let y = !r2 in
+     r1 := y;
+     r2 := x)
 
-//      <: STATE unit (fun post m -> m == ((r1 |> x) <*> (r2 |> y)) /\ (defined m /\ post () ((r1 |> y) <*> (r2 |> x))))
+     <: STATE unit (fun post m -> m == ((r1 |> x) <*> (r2 |> y)) /\ (defined m /\ post () ((r1 |> y) <*> (r2 |> x))))
 
-//      by (fun () -> prelude ();
-//                 process_command ();
-// 		get_to_the_next_frame ();
-// 		process_command ();
-// 	        apply_lemma (`lemma_rewrite_sep_comm);
-// 		process_command ();
-// 	        get_to_the_next_frame ();
-// 		process_command ();
-// 	        apply_lemma (`lemma_rewrite_sep_comm);
-// 		process_command ();
-// 	        get_to_the_next_frame ();
-// 	        apply_lemma (`lemma_rewrite_sep_comm);
-// 		process_command ())
+     by sl' // (fun () -> prelude ();
+//             //     process_command ();
+// 	    //     get_to_the_next_frame ();
+// 	    //     process_command ();
+// 	    //     apply_lemma (`lemma_rewrite_sep_comm);
+// 	    //     process_command ();
+// 	    //     get_to_the_next_frame ();
+// 	    //     process_command ();
+// 	    //     apply_lemma (`lemma_rewrite_sep_comm);
+// 	    //     process_command ();
+// 	    //     get_to_the_next_frame ();
+// 	    //     apply_lemma (`lemma_rewrite_sep_comm);
+// 	    //     process_command ())
 
-// (*
-//  * three commands, the inline pure expressions don't count
-//  *)
-// let incr (r:ref int) (x:int)
-//   = (let y = !r in
-//      let z = y + 1 in
-//      r := z;
-//      !r)
+// // (*
+// //  * three commands, the inline pure expressions don't count
+// //  *)
+// // let incr (r:ref int) (x:int)
+// //   = (let y = !r in
+// //      let z = y + 1 in
+// //      r := z;
+// //      !r)
 
-//      <: STATE int (fun post m -> m == (r |> x) /\ (defined m /\ post (x + 1) (r |> x + 1)))
+// //      <: STATE int (fun post m -> m == (r |> x) /\ (defined m /\ post (x + 1) (r |> x + 1)))
 
-//      by (fun () -> prelude ();
-//                 process_command ();
-// 		get_to_the_next_frame ();
-// 		process_command ();
-// 		get_to_the_next_frame ();
-// 		process_command ();
-// 		get_to_the_next_frame ();
-// 		process_command ())
+// //      by (fun () -> prelude ();
+// //                 process_command ();
+// // 		get_to_the_next_frame ();
+// // 		process_command ();
+// // 		get_to_the_next_frame ();
+// // 		process_command ();
+// // 		get_to_the_next_frame ();
+// // 		process_command ())
 
-// (*
-//  * 2 commands
-//  *)
-// let incr2 (r:ref int) (x:int)
-//   = (let y = incr r x in
-//      incr r y)
+// // (*
+// //  * 2 commands
+// //  *)
+// // let incr2 (r:ref int) (x:int)
+// //   = (let y = incr r x in
+// //      incr r y)
 
-//     <: STATE int (fun post m -> m == (r |> x) /\ (defined m /\ post (x + 2) (r |> x + 2)))
+// //     <: STATE int (fun post m -> m == (r |> x) /\ (defined m /\ post (x + 2) (r |> x + 2)))
 
-//     by (fun () -> prelude ();
-//                process_command ();
-// 	       get_to_the_next_frame ();
-// 	       process_command ())
+// //     by (fun () -> prelude ();
+// //                process_command ();
+// // 	       get_to_the_next_frame ();
+// // 	       process_command ())
 
-// let rotate (r1 r2 r3:ref int) (x y z:int) =
-//   (swap r2 r3 y z;
-//    swap r1 r2 x z;
-//    let x = !r1 in
-//    x)
+// // let rotate (r1 r2 r3:ref int) (x y z:int) =
+// //   (swap r2 r3 y z;
+// //    swap r1 r2 x z;
+// //    let x = !r1 in
+// //    x)
    
-//   <: STATE int (fun post m -> m == ((r1 |> x) <*> ((r2 |> y) <*> (r3 |> z))) /\
-//                          (defined m /\ post z ((r1 |> z) <*> ((r2 |> x) <*> (r3 |> y)))))
+// //   <: STATE int (fun post m -> m == ((r1 |> x) <*> ((r2 |> y) <*> (r3 |> z))) /\
+// //                          (defined m /\ post z ((r1 |> z) <*> ((r2 |> x) <*> (r3 |> y)))))
 
-//   by (fun () -> prelude ();
-//              apply_lemma (`lemma_rewrite_sep_comm);
-//              process_command ();
-// 	     get_to_the_next_frame ();
-// 	     process_command ();
-// 	     apply_lemma (`lemma_rewrite_sep_comm);
-// 	     apply_lemma (`lemma_rewrite_sep_assoc3);
-// 	     process_command ();
-// 	     get_to_the_next_frame ();
-// 	     apply_lemma (`lemma_rewrite_sep_assoc4);
-// 	     process_command ();
-// 	     process_command ();
-// 	     get_to_the_next_frame ();
-// 	     process_command ())
+// //   by (fun () -> prelude ();
+// //              apply_lemma (`lemma_rewrite_sep_comm);
+// //              process_command ();
+// // 	     get_to_the_next_frame ();
+// // 	     process_command ();
+// // 	     apply_lemma (`lemma_rewrite_sep_comm);
+// // 	     apply_lemma (`lemma_rewrite_sep_assoc3);
+// // 	     process_command ();
+// // 	     get_to_the_next_frame ();
+// // 	     apply_lemma (`lemma_rewrite_sep_assoc4);
+// // 	     process_command ();
+// // 	     process_command ();
+// // 	     get_to_the_next_frame ();
+// // 	     process_command ())
 
-// let lemma_inline_in_patterns_two (psi1 psi2:Type) (m m':memory) (phi1 phi2: memory -> memory -> Type)
-//   :Lemma (requires (defined (m <*> m') /\ ((psi1 ==> phi1 (m <*> m') emp) /\ (psi2 ==> phi2 (m <*> m') emp))))
-//          (ensures  (exists (m0 m1:memory). defined (m0 <*> m1) /\ (m <*> m') == (m0 <*> m1) /\
-// 	                              ((psi1 ==> phi1 m0 m1) /\
-// 				       (psi2 ==> phi2 m0 m1))))
-//   = ()
+// // let lemma_inline_in_patterns_two (psi1 psi2:Type) (m m':memory) (phi1 phi2: memory -> memory -> Type)
+// //   :Lemma (requires (defined (m <*> m') /\ ((psi1 ==> phi1 (m <*> m') emp) /\ (psi2 ==> phi2 (m <*> m') emp))))
+// //          (ensures  (exists (m0 m1:memory). defined (m0 <*> m1) /\ (m <*> m') == (m0 <*> m1) /\
+// // 	                              ((psi1 ==> phi1 m0 m1) /\
+// // 				       (psi2 ==> phi2 m0 m1))))
+// //   = ()
 
-// let lemma_frame_out_empty_right (phi:memory -> memory -> memory -> Type) (m:memory)
-//   :Lemma (requires (defined m /\ phi m m emp))
-//          (ensures  (exists (m0 m1:memory). defined (m0 <*> m1) /\ m == (m0 <*> m1) /\ phi m m0 m1))
-//   = ()
+// // let lemma_frame_out_empty_right (phi:memory -> memory -> memory -> Type) (m:memory)
+// //   :Lemma (requires (defined m /\ phi m m emp))
+// //          (ensures  (exists (m0 m1:memory). defined (m0 <*> m1) /\ m == (m0 <*> m1) /\ phi m m0 m1))
+// //   = ()
 
-// let lemma_frame_out_empty_left (phi:memory -> memory -> memory -> Type) (m:memory)
-//   :Lemma (requires (defined m /\ phi m emp m))
-//          (ensures  (exists (m0 m1:memory). defined (m0 <*> m1) /\ m == (m0 <*> m1) /\ phi m m0 m1))
-//   = lemma_sep_comm m emp
+// // let lemma_frame_out_empty_left (phi:memory -> memory -> memory -> Type) (m:memory)
+// //   :Lemma (requires (defined m /\ phi m emp m))
+// //          (ensures  (exists (m0 m1:memory). defined (m0 <*> m1) /\ m == (m0 <*> m1) /\ phi m m0 m1))
+// //   = lemma_sep_comm m emp
 
-// let cond_test (r1 r2:ref int) (x:int) (b:bool)
-//   = (let y = !r1 in
-//      match b with
-//      | true  -> r1 := y + 1
-//      | false -> r2 := y + 2)
+// // let cond_test (r1 r2:ref int) (x:int) (b:bool)
+// //   = (let y = !r1 in
+// //      match b with
+// //      | true  -> r1 := y + 1
+// //      | false -> r2 := y + 2)
 
-//     <: STATE unit (fun p m -> m == ((r1 |> x) <*> (r2 |> x)) /\ (defined m /\ (b ==> p () ((r1 |> x + 1) <*> (r2 |> x))) /\
-//                                                                        (~ b ==> p () ((r1 |> x) <*> (r2 |> x + 2)))))
+// //     <: STATE unit (fun p m -> m == ((r1 |> x) <*> (r2 |> x)) /\ (defined m /\ (b ==> p () ((r1 |> x + 1) <*> (r2 |> x))) /\
+// //                                                                        (~ b ==> p () ((r1 |> x) <*> (r2 |> x + 2)))))
 
-//     by (fun () -> prelude ();
-//                apply_lemma (`lemma_rw);
-// 	       get_to_the_next_frame ();
-// 	       apply_lemma (`lemma_inline_in_patterns_two);
-// 	       split (); smt ();
-// 	       split ();
-// 	       //goal 1
-// 	       ignore (implies_intro ());
-// 	       apply_lemma (`lemma_rw);
-// 	       split (); smt (); split (); smt ();
-// 	       apply_lemma (`lemma_pure_right);
-// 	       smt ();
-// 	       //goal 2
-// 	       ignore (implies_intro ());
-// 	       apply_lemma (`lemma_frame_out_empty_right);
-// 	       split (); smt ();
-// 	       split ();
-// 	       //goal 2.1
-// 	       ignore (implies_intro ());
-// 	       apply_lemma (`lemma_rewrite_sep_comm);
-// 	       apply_lemma (`lemma_rw);
-// 	       split (); smt ();
-// 	       split (); smt ();
-// 	       apply_lemma (`lemma_frame_out_empty_left);
-// 	       split (); smt (); split (); smt (); split (); smt ();
-// 	       apply_lemma (`lemma_frame_out_empty_left);
-// 	       smt ();
-// 	       //goal 2.2
-// 	       smt ())
+// //     by (fun () -> prelude ();
+// //                apply_lemma (`lemma_rw);
+// // 	       get_to_the_next_frame ();
+// // 	       apply_lemma (`lemma_inline_in_patterns_two);
+// // 	       split (); smt ();
+// // 	       split ();
+// // 	       //goal 1
+// // 	       ignore (implies_intro ());
+// // 	       apply_lemma (`lemma_rw);
+// // 	       split (); smt (); split (); smt ();
+// // 	       apply_lemma (`lemma_pure_right);
+// // 	       smt ();
+// // 	       //goal 2
+// // 	       ignore (implies_intro ());
+// // 	       apply_lemma (`lemma_frame_out_empty_right);
+// // 	       split (); smt ();
+// // 	       split ();
+// // 	       //goal 2.1
+// // 	       ignore (implies_intro ());
+// // 	       apply_lemma (`lemma_rewrite_sep_comm);
+// // 	       apply_lemma (`lemma_rw);
+// // 	       split (); smt ();
+// // 	       split (); smt ();
+// // 	       apply_lemma (`lemma_frame_out_empty_left);
+// // 	       split (); smt (); split (); smt (); split (); smt ();
+// // 	       apply_lemma (`lemma_frame_out_empty_left);
+// // 	       smt ();
+// // 	       //goal 2.2
+// // 	       smt ())
 
-// #reset-options "--print_full_names --__no_positivity"
+// // #reset-options "--print_full_names --__no_positivity"
 
-// noeq type listcell =
-//   | Cell :head:int -> tail:listptr -> listcell
+// // noeq type listcell =
+// //   | Cell :head:int -> tail:listptr -> listcell
 
-// and listptr = option (ref listcell)
+// // and listptr = option (ref listcell)
 
-// #reset-options "--print_full_names --__temp_fast_implicits"
+// // #reset-options "--print_full_names --__temp_fast_implicits"
 
-// let rec valid (p:listptr) (repr:list int) (m:memory) :Tot Type0 (decreases repr) =
-//   defined m /\
-//   (match repr with
-//    | []    -> None? p /\ m == emp
-//    | hd::tl -> Some? p /\
-//              (exists (tail:listptr) (m1:memory). m == (((Some?.v p) |> Cell hd tail) <*> m1) /\ valid tail tl m1))
+// // let rec valid (p:listptr) (repr:list int) (m:memory) :Tot Type0 (decreases repr) =
+// //   defined m /\
+// //   (match repr with
+// //    | []    -> None? p /\ m == emp
+// //    | hd::tl -> Some? p /\
+// //              (exists (tail:listptr) (m1:memory). m == (((Some?.v p) |> Cell hd tail) <*> m1) /\ valid tail tl m1))
                                                       
-// private let __exists_elim_as_forall2
-//   (#a:Type) (#b:Type) (#p: a -> b -> Type) (#phi:Type)
-//   (_:(exists x y. p x y)) (_:(squash (forall (x:a) (y:b). p x y ==> phi)))
-//   :Lemma phi
-//   = ()
-
-// private let __exists_elim_as_forall1
-//   (#a:Type) (#p:a -> Type) (#phi:Type)
-//   (_:(exists x. p x)) (_:(squash (forall (x:a). p x ==> phi)))
-//   :Lemma phi
-//   = ()
-
-// private let __elim_and (h:binder) :Tac unit
-//   = and_elim (pack (Tv_Var (bv_of_binder h)));
-//     clear h
-
-// private let __elim_exists1 (h:binder) :Tac unit
-//   = let t = `__exists_elim_as_forall1 in
-//     apply_lemma (mk_e_app t [pack (Tv_Var (bv_of_binder h))]);
-//     clear h;
-//     ignore (forall_intros ())
-
-// private let __elim_exists_return_binders2 (h:binder) :Tac (list binder)
-//   = let t = `__exists_elim_as_forall2 in
-//     apply_lemma (mk_e_app t [pack (Tv_Var (bv_of_binder h))]);
-//     clear h;
-//     forall_intros ()
-
-// private let __elim_exists2 (h:binder) :Tac unit = ignore (__elim_exists_return_binders2 h)
-
-// (*
-//  * AR: these two lemmas are useless because of no match-ing in the unifier
-//  *)
-// // #set-options "--z3rlimit 30"
-// // private let __elim_list_match0 (#a:Type) (l:list a) (phi:Type) (psi:a -> list a -> Type) (rest:list a -> Type)
-// //   :Lemma (requires (((l == [] /\ phi) ==> rest []) /\
-// //                     (forall hd tl. (l == Cons hd tl /\ psi hd tl) ==> rest (Cons hd tl))))
-// //          (ensures  ((match l with
-// // 	             | []         -> phi
-// // 		     | Cons hd tl -> psi hd tl) ==> rest l))
+// // private let __exists_elim_as_forall2
+// //   (#a:Type) (#b:Type) (#p: a -> b -> Type) (#phi:Type)
+// //   (_:(exists x y. p x y)) (_:(squash (forall (x:a) (y:b). p x y ==> phi)))
+// //   :Lemma phi
 // //   = ()
 
-// // private let __list_match_elim_as_cases (#l:list int) (#phi:list int -> Type0) (#psi:list int -> int -> list int -> Type0) (#rest:list int -> Type0)
-// //   (_:(match l with
-// //       | []         -> phi l
-// //       | Cons hd tl -> psi l hd tl))
-// //   (_:squash (((l == [] /\ phi []) ==> rest []) /\
-// //              ((forall hd tl. (l == Cons hd tl /\ psi (Cons hd tl) hd tl) ==> rest (Cons hd tl)))))
-// //   :Lemma (rest l)
+// // private let __exists_elim_as_forall1
+// //   (#a:Type) (#p:a -> Type) (#phi:Type)
+// //   (_:(exists x. p x)) (_:(squash (forall (x:a). p x ==> phi)))
+// //   :Lemma phi
 // //   = ()
 
-// // private let __elim_list_match (h:binder) :Tac unit
-// //   = let t = `__list_match_elim_as_cases in
-// //     apply_lemma (mk_e_app t [pack (Tv_Var (bv_of_binder h))])
-// //     //clear h
+// // private let __elim_and (h:binder) :Tac unit
+// //   = and_elim (pack (Tv_Var (bv_of_binder h)));
+// //     clear h
 
-// //i tried a style where i pass the proof of valid p repr m as a squashed term
-// //but even then unification fails
-// //currently all the arguments have to be provided explicitly
-// let __elim_valid_without_match
-//   (#p:listptr) (#repr:list int) (#m:memory) (#goal:listptr -> list int -> memory -> Type0)
-//   :Lemma (requires ((valid p repr m) /\
-//                     (((repr == [] /\ p == None /\ m == emp) ==> goal None [] emp) /\
-//                      (forall hd tl. (repr == hd::tl /\
-// 	                        Some? p       /\
-// 			        (exists tail m1. m == (((Some?.v p) |> Cell hd tail) <*> m1) /\ valid tail tl m1))
-// 		               ==> goal p (Cons hd tl) m))))
-//          (ensures  (goal p repr m))
-//   = admit ()
+// // private let __elim_exists1 (h:binder) :Tac unit
+// //   = let t = `__exists_elim_as_forall1 in
+// //     apply_lemma (mk_e_app t [pack (Tv_Var (bv_of_binder h))]);
+// //     clear h;
+// //     ignore (forall_intros ())
 
-// let lemma_frame_exact (phi:memory -> memory -> memory -> memory -> Type0) (h h':memory)
-//   :Lemma (requires (defined (h <*> h') /\ phi h h' h h'))
-//          (ensures  (exists (h0 h1:memory). defined (h0 <*> h1) /\ (h <*> h') == (h0 <*> h1) /\ phi h h' h0 h1))
-//   = ()
+// // private let __elim_exists_return_binders2 (h:binder) :Tac (list binder)
+// //   = let t = `__exists_elim_as_forall2 in
+// //     apply_lemma (mk_e_app t [pack (Tv_Var (bv_of_binder h))]);
+// //     clear h;
+// //     forall_intros ()
 
-// let rec length (l:listptr)
-//   = (match l with
-//      | None   -> (0 <: STATE int (fun p h -> p 0 emp))
-//      | Some r ->
-//        let Cell hd tl = !r in
-//        1 + length tl)
+// // private let __elim_exists2 (h:binder) :Tac unit = ignore (__elim_exists_return_binders2 h)
 
-//     <: STATE int (fun p m -> exists (fl:list int). valid l fl m /\ p (List.Tot.length fl) m)
+// // (*
+// //  * AR: these two lemmas are useless because of no match-ing in the unifier
+// //  *)
+// // // #set-options "--z3rlimit 30"
+// // // private let __elim_list_match0 (#a:Type) (l:list a) (phi:Type) (psi:a -> list a -> Type) (rest:list a -> Type)
+// // //   :Lemma (requires (((l == [] /\ phi) ==> rest []) /\
+// // //                     (forall hd tl. (l == Cons hd tl /\ psi hd tl) ==> rest (Cons hd tl))))
+// // //          (ensures  ((match l with
+// // // 	             | []         -> phi
+// // // 		     | Cons hd tl -> psi hd tl) ==> rest l))
+// // //   = ()
 
-//     by (fun _ -> ignore (forall_intros ());
-//               let h = implies_intro () in __elim_exists1 h;
-// 	      let h = implies_intro () in __elim_and h;
-// 	      ignore (implies_intro ());
-// 	      apply_lemma (`__elim_valid_without_match);  //this is fragile
-// 	      assumption (); assumption (); assumption ();
-// 	      split (); smt ();
-// 	      split ();
-// 	      let h = implies_intro () in __elim_and h;
-// 	      let h = implies_intro () in __elim_and h;
-// 	      let h = implies_intro () in rewrite h; let h = implies_intro () in rewrite h;
-//               let h = implies_intro () in rewrite h;
-// 	      ignore (implies_intro ());
-// 	      split ();
-// 	      ignore (implies_intro ());
-// 	      apply_lemma (`lemma_frame_out_empty_left);
-// 	      split (); smt ();
-// 	      ignore (implies_intro ());
-// 	      split (); smt (); split (); smt ();
-// 	      apply_lemma (`lemma_frame_out_empty_left);
-// 	      smt (); smt ();
+// // // private let __list_match_elim_as_cases (#l:list int) (#phi:list int -> Type0) (#psi:list int -> int -> list int -> Type0) (#rest:list int -> Type0)
+// // //   (_:(match l with
+// // //       | []         -> phi l
+// // //       | Cons hd tl -> psi l hd tl))
+// // //   (_:squash (((l == [] /\ phi []) ==> rest []) /\
+// // //              ((forall hd tl. (l == Cons hd tl /\ psi (Cons hd tl) hd tl) ==> rest (Cons hd tl)))))
+// // //   :Lemma (rest l)
+// // //   = ()
 
-//               //inductive case
-// 	      let hd_binder = forall_intro () in
-// 	      let tl_binder = forall_intro () in
-// 	      let h = implies_intro () in __elim_and h;
-// 	      let h = implies_intro () in __elim_and h;
-// 	      let h = implies_intro () in rewrite h;
-// 	      ignore (implies_intro ());
-// 	      let h = implies_intro () in __elim_exists2 h;
-// 	      let h = implies_intro () in __elim_and h;
-// 	      let h = implies_intro () in rewrite h;
-// 	      ignore (implies_intros ());
-// 	      split (); smt ();
+// // // private let __elim_list_match (h:binder) :Tac unit
+// // //   = let t = `__list_match_elim_as_cases in
+// // //     apply_lemma (mk_e_app t [pack (Tv_Var (bv_of_binder h))])
+// // //     //clear h
 
-//               ignore (implies_intro ());
-// 	      apply_lemma (`lemma_inline_in_patterns_two);
-// 	      split (); smt ();
-// 	      split ();
-// 	      ignore (implies_intro ());
-// 	      apply_lemma (`lemma_frame_out_empty_right);
-// 	      split (); smt ();
-// 	      ignore (forall_intro ());
-// 	      let h = implies_intro () in rewrite h;
-// 	      norm [delta_only ["FStar.Pervasives.Native.__proj__Some__item__v"]];
-// 	      apply_lemma (`lemma_rw);
-// 	      split (); smt ();
-// 	      split (); smt ();
-// 	      apply_lemma (`lemma_frame_out_empty_right);
-// 	      split (); smt ();
-// 	      apply_lemma (`lemma_frame_out_empty_right);
-// 	      split (); smt ();
-// 	      ignore (forall_intros ()); ignore (implies_intro ());
-// 	      apply_lemma (`lemma_rewrite_sep_comm);
-// 	      apply_lemma (`lemma_frame_exact);
-// 	      split (); smt ();
-// 	      let w = let bv, _ = inspect_binder tl_binder in pack (Tv_Var bv) in
-// 	      witness w;
-// 	      split (); smt (); split (); smt ();
-// 	      apply_lemma (`lemma_frame_out_empty_left);
-// 	      split (); smt ();
-// 	      ignore (forall_intro ());
-// 	      ignore (implies_intro ());
-// 	      split (); smt (); split (); smt ();
-// 	      apply_lemma (`lemma_frame_out_empty_left);
-// 	      split (); smt (); split (); smt ();
-// 	      split (); smt (); split (); smt ();
-// 	      apply_lemma (`lemma_frame_out_empty_left);
-// 	      split (); smt (); split (); smt (); split (); smt ();
-// 	      apply_lemma (`lemma_frame_out_empty_left);
-// 	      smt ();
-// 	      smt ())
+// // //i tried a style where i pass the proof of valid p repr m as a squashed term
+// // //but even then unification fails
+// // //currently all the arguments have to be provided explicitly
+// // let __elim_valid_without_match
+// //   (#p:listptr) (#repr:list int) (#m:memory) (#goal:listptr -> list int -> memory -> Type0)
+// //   :Lemma (requires ((valid p repr m) /\
+// //                     (((repr == [] /\ p == None /\ m == emp) ==> goal None [] emp) /\
+// //                      (forall hd tl. (repr == hd::tl /\
+// // 	                        Some? p       /\
+// // 			        (exists tail m1. m == (((Some?.v p) |> Cell hd tail) <*> m1) /\ valid tail tl m1))
+// // 		               ==> goal p (Cons hd tl) m))))
+// //          (ensures  (goal p repr m))
+// //   = admit ()
+
+// // let lemma_frame_exact (phi:memory -> memory -> memory -> memory -> Type0) (h h':memory)
+// //   :Lemma (requires (defined (h <*> h') /\ phi h h' h h'))
+// //          (ensures  (exists (h0 h1:memory). defined (h0 <*> h1) /\ (h <*> h') == (h0 <*> h1) /\ phi h h' h0 h1))
+// //   = ()
+
+// // let rec length (l:listptr)
+// //   = (match l with
+// //      | None   -> (0 <: STATE int (fun p h -> p 0 emp))
+// //      | Some r ->
+// //        let Cell hd tl = !r in
+// //        1 + length tl)
+
+// //     <: STATE int (fun p m -> exists (fl:list int). valid l fl m /\ p (List.Tot.length fl) m)
+
+// //     by (fun _ -> ignore (forall_intros ());
+// //               let h = implies_intro () in __elim_exists1 h;
+// // 	      let h = implies_intro () in __elim_and h;
+// // 	      ignore (implies_intro ());
+// // 	      apply_lemma (`__elim_valid_without_match);  //this is fragile
+// // 	      assumption (); assumption (); assumption ();
+// // 	      split (); smt ();
+// // 	      split ();
+// // 	      let h = implies_intro () in __elim_and h;
+// // 	      let h = implies_intro () in __elim_and h;
+// // 	      let h = implies_intro () in rewrite h; let h = implies_intro () in rewrite h;
+// //               let h = implies_intro () in rewrite h;
+// // 	      ignore (implies_intro ());
+// // 	      split ();
+// // 	      ignore (implies_intro ());
+// // 	      apply_lemma (`lemma_frame_out_empty_left);
+// // 	      split (); smt ();
+// // 	      ignore (implies_intro ());
+// // 	      split (); smt (); split (); smt ();
+// // 	      apply_lemma (`lemma_frame_out_empty_left);
+// // 	      smt (); smt ();
+
+// //               //inductive case
+// // 	      let hd_binder = forall_intro () in
+// // 	      let tl_binder = forall_intro () in
+// // 	      let h = implies_intro () in __elim_and h;
+// // 	      let h = implies_intro () in __elim_and h;
+// // 	      let h = implies_intro () in rewrite h;
+// // 	      ignore (implies_intro ());
+// // 	      let h = implies_intro () in __elim_exists2 h;
+// // 	      let h = implies_intro () in __elim_and h;
+// // 	      let h = implies_intro () in rewrite h;
+// // 	      ignore (implies_intros ());
+// // 	      split (); smt ();
+
+// //               ignore (implies_intro ());
+// // 	      apply_lemma (`lemma_inline_in_patterns_two);
+// // 	      split (); smt ();
+// // 	      split ();
+// // 	      ignore (implies_intro ());
+// // 	      apply_lemma (`lemma_frame_out_empty_right);
+// // 	      split (); smt ();
+// // 	      ignore (forall_intro ());
+// // 	      let h = implies_intro () in rewrite h;
+// // 	      norm [delta_only ["FStar.Pervasives.Native.__proj__Some__item__v"]];
+// // 	      apply_lemma (`lemma_rw);
+// // 	      split (); smt ();
+// // 	      split (); smt ();
+// // 	      apply_lemma (`lemma_frame_out_empty_right);
+// // 	      split (); smt ();
+// // 	      apply_lemma (`lemma_frame_out_empty_right);
+// // 	      split (); smt ();
+// // 	      ignore (forall_intros ()); ignore (implies_intro ());
+// // 	      apply_lemma (`lemma_rewrite_sep_comm);
+// // 	      apply_lemma (`lemma_frame_exact);
+// // 	      split (); smt ();
+// // 	      let w = let bv, _ = inspect_binder tl_binder in pack (Tv_Var bv) in
+// // 	      witness w;
+// // 	      split (); smt (); split (); smt ();
+// // 	      apply_lemma (`lemma_frame_out_empty_left);
+// // 	      split (); smt ();
+// // 	      ignore (forall_intro ());
+// // 	      ignore (implies_intro ());
+// // 	      split (); smt (); split (); smt ();
+// // 	      apply_lemma (`lemma_frame_out_empty_left);
+// // 	      split (); smt (); split (); smt ();
+// // 	      split (); smt (); split (); smt ();
+// // 	      apply_lemma (`lemma_frame_out_empty_left);
+// // 	      split (); smt (); split (); smt (); split (); smt ();
+// // 	      apply_lemma (`lemma_frame_out_empty_left);
+// // 	      smt ();
+// // 	      smt ())
 
 
-// let binder_to_term b = let bv, _ = inspect_binder b in pack (Tv_Var bv)
+// // let binder_to_term b = let bv, _ = inspect_binder b in pack (Tv_Var bv)
 
-// //#set-options "--admit_smt_queries true"
-// //#set-options "--z3rlimit 30"
-// let rec append (l1 l2:listptr)
-//   = (match l1 with
-//      | None   -> l2
-//      | Some r ->
-//        let Cell hd tl = !r in
-//        match tl with
-//        | Some tl_r ->
-//          let rest = append tl l2 in
-// 	 l1
-//        | None ->
-//          r := Cell hd l2;
-// 	 l1)
+// // //#set-options "--admit_smt_queries true"
+// // //#set-options "--z3rlimit 30"
+// // let rec append (l1 l2:listptr)
+// //   = (match l1 with
+// //      | None   -> l2
+// //      | Some r ->
+// //        let Cell hd tl = !r in
+// //        match tl with
+// //        | Some tl_r ->
+// //          let rest = append tl l2 in
+// // 	 l1
+// //        | None ->
+// //          r := Cell hd l2;
+// // 	 l1)
 
-//      <: STATE listptr (fun p m -> exists (fl1 fl2:list int) (m1 m2:memory).
-//                                  defined (m1 <*> m2) /\
-// 				 m == (m1 <*> m2)    /\
-// 				 valid l1 fl1 m1     /\
-// 				 valid l2 fl2 m2     /\
-// 				 (forall mf l. ((Set.equal (addrs_in mf) (Set.union (addrs_in m1) (addrs_in m2))) /\
-// 				           (Some? l1 ==> l1 == l)                                             /\
-// 				           (valid l (List.Tot.append fl1 fl2) mf)) ==> p l mf))
+// //      <: STATE listptr (fun p m -> exists (fl1 fl2:list int) (m1 m2:memory).
+// //                                  defined (m1 <*> m2) /\
+// // 				 m == (m1 <*> m2)    /\
+// // 				 valid l1 fl1 m1     /\
+// // 				 valid l2 fl2 m2     /\
+// // 				 (forall mf l. ((Set.equal (addrs_in mf) (Set.union (addrs_in m1) (addrs_in m2))) /\
+// // 				           (Some? l1 ==> l1 == l)                                             /\
+// // 				           (valid l (List.Tot.append fl1 fl2) mf)) ==> p l mf))
 
-//      by (fun () -> ignore (forall_intros ());
-//                 let h = implies_intro () in
-// 		let l = __elim_exists_return_binders2 h in
-// 		let fl1_binder = List.Tot.hd l in
-// 		let fl2_binder = List.Tot.hd (List.Tot.tl l) in
-//                 let h = implies_intro () in
-// 		let l = __elim_exists_return_binders2 h in
-// 		let m1_binder = List.Tot.hd l in
-// 		let m2_binder = List.Tot.hd (List.Tot.tl l) in
-// 		let h = implies_intro () in __elim_and h;
-// 		let h = implies_intro () in __elim_and h;
-// 		let h = implies_intro () in __elim_and h;
-// 		let h = implies_intro () in __elim_and h;
-// 		ignore (implies_intro ());
-// 		let h = implies_intro () in rewrite h;
-// 		ignore (implies_intro ());
+// //      by (fun () -> ignore (forall_intros ());
+// //                 let h = implies_intro () in
+// // 		let l = __elim_exists_return_binders2 h in
+// // 		let fl1_binder = List.Tot.hd l in
+// // 		let fl2_binder = List.Tot.hd (List.Tot.tl l) in
+// //                 let h = implies_intro () in
+// // 		let l = __elim_exists_return_binders2 h in
+// // 		let m1_binder = List.Tot.hd l in
+// // 		let m2_binder = List.Tot.hd (List.Tot.tl l) in
+// // 		let h = implies_intro () in __elim_and h;
+// // 		let h = implies_intro () in __elim_and h;
+// // 		let h = implies_intro () in __elim_and h;
+// // 		let h = implies_intro () in __elim_and h;
+// // 		ignore (implies_intro ());
+// // 		let h = implies_intro () in rewrite h;
+// // 		ignore (implies_intro ());
 
-//                 //induction on fl1
-// 		apply_lemma (`__elim_valid_without_match);
-// 		exact (quote l1);
-// 		exact (binder_to_term fl1_binder);
-// 		exact (binder_to_term m1_binder);
-// 		split (); smt ();  //this is the extra valid goal from __elim_valid_without_match
+// //                 //induction on fl1
+// // 		apply_lemma (`__elim_valid_without_match);
+// // 		exact (quote l1);
+// // 		exact (binder_to_term fl1_binder);
+// // 		exact (binder_to_term m1_binder);
+// // 		split (); smt ();  //this is the extra valid goal from __elim_valid_without_match
 
-//                 split ();
+// //                 split ();
 
-//                 //empty fl1 case
-// 		let h = implies_intro () in __elim_and h;
-// 		let h = implies_intro () in __elim_and h;
-// 		let h = implies_intro () in rewrite h;
-// 		let h = implies_intro () in rewrite h;
-// 		let h = implies_intro () in rewrite h;
+// //                 //empty fl1 case
+// // 		let h = implies_intro () in __elim_and h;
+// // 		let h = implies_intro () in __elim_and h;
+// // 		let h = implies_intro () in rewrite h;
+// // 		let h = implies_intro () in rewrite h;
+// // 		let h = implies_intro () in rewrite h;
 
-//                 ignore (implies_intro ()); //the valid assumption for l2
-// 		ignore (implies_intro ()); //this is the foall mf f. assumption, keep an eye on it
+// //                 ignore (implies_intro ()); //the valid assumption for l2
+// // 		ignore (implies_intro ()); //this is the foall mf f. assumption, keep an eye on it
 
-//                 split ();
+// //                 split ();
 
-//                 ignore (implies_intro ());
-// 		apply_lemma (`lemma_frame_out_empty_left);
-// 		split (); smt ();
-// 		ignore (implies_intro ()); ignore (forall_intro ()); ignore (implies_intro ()); ignore (forall_intro ()); ignore (implies_intro ());
-// 		split (); smt ();
-// 		apply_lemma (`lemma_frame_out_empty_left);
-// 		smt ();
+// //                 ignore (implies_intro ());
+// // 		apply_lemma (`lemma_frame_out_empty_left);
+// // 		split (); smt ();
+// // 		ignore (implies_intro ()); ignore (forall_intro ()); ignore (implies_intro ()); ignore (forall_intro ()); ignore (implies_intro ());
+// // 		split (); smt ();
+// // 		apply_lemma (`lemma_frame_out_empty_left);
+// // 		smt ();
 
-//                 //inconsistent ()
-// 		ignore (implies_intro ());
-// 		smt ();
+// //                 //inconsistent ()
+// // 		ignore (implies_intro ());
+// // 		smt ();
 
-//                 //inductive case fl1 is Cons
+// //                 //inductive case fl1 is Cons
 
-//                 let fl1_head = forall_intro () in
-// 		let fl1_tail = forall_intro () in
-// 		let h = implies_intro () in __elim_and h;
-// 		let h = implies_intro () in __elim_and h;
-// 		let h = implies_intro () in rewrite h;
-// 		ignore (implies_intro ());
-// 		let h = implies_intro () in let l1 = __elim_exists_return_binders2 h in
-// 		let l1_tail = List.Tot.hd l1 in
-// 		let l1_tail_memory = List.Tot.hd (List.Tot.tl l1) in
-// 		let h = implies_intro () in __elim_and h;
-// 		let h = implies_intro () in rewrite h;
-// 		ignore (implies_intro ());
-// 		ignore (implies_intro ());
+// //                 let fl1_head = forall_intro () in
+// // 		let fl1_tail = forall_intro () in
+// // 		let h = implies_intro () in __elim_and h;
+// // 		let h = implies_intro () in __elim_and h;
+// // 		let h = implies_intro () in rewrite h;
+// // 		ignore (implies_intro ());
+// // 		let h = implies_intro () in let l1 = __elim_exists_return_binders2 h in
+// // 		let l1_tail = List.Tot.hd l1 in
+// // 		let l1_tail_memory = List.Tot.hd (List.Tot.tl l1) in
+// // 		let h = implies_intro () in __elim_and h;
+// // 		let h = implies_intro () in rewrite h;
+// // 		ignore (implies_intro ());
+// // 		ignore (implies_intro ());
 
-//                 ignore (implies_intro ()); //this is the forall mf f. assumption, keep an eye on it
+// //                 ignore (implies_intro ()); //this is the forall mf f. assumption, keep an eye on it
 
-//                 split ();
+// //                 split ();
 
-//                 //inconsistent
-//                 ignore (implies_intro ());
-// 		smt ();
+// //                 //inconsistent
+// //                 ignore (implies_intro ());
+// // 		smt ();
 
-//                 ignore (implies_intro ());
-// 		apply_lemma (`lemma_inline_in_patterns_two);
-// 		split (); smt ();
+// //                 ignore (implies_intro ());
+// // 		apply_lemma (`lemma_inline_in_patterns_two);
+// // 		split (); smt ();
 
-//                 split ();
+// //                 split ();
 
-//                 ignore (implies_intro ());
-// 		apply_lemma (`lemma_frame_out_empty_right);
-// 		split (); smt ();
+// //                 ignore (implies_intro ());
+// // 		apply_lemma (`lemma_frame_out_empty_right);
+// // 		split (); smt ();
 
-//                 ignore (forall_intro ());
-// 		let h = implies_intro () in rewrite h;
-// 	        norm [delta_only ["FStar.Pervasives.Native.__proj__Some__item__v"]];
-// 		apply_lemma (`lemma_rewrite_sep_assoc4);
-// 		apply_lemma (`lemma_rw);
-// 		split (); smt (); split (); smt ();
-// 		apply_lemma (`lemma_frame_out_empty_right);
-// 		split (); smt ();
-// 		apply_lemma (`lemma_frame_out_empty_right);
-// 		split (); smt ();
-//                 ignore (forall_intros ()); ignore (implies_intro ());
+// //                 ignore (forall_intro ());
+// // 		let h = implies_intro () in rewrite h;
+// // 	        norm [delta_only ["FStar.Pervasives.Native.__proj__Some__item__v"]];
+// // 		apply_lemma (`lemma_rewrite_sep_assoc4);
+// // 		apply_lemma (`lemma_rw);
+// // 		split (); smt (); split (); smt ();
+// // 		apply_lemma (`lemma_frame_out_empty_right);
+// // 		split (); smt ();
+// // 		apply_lemma (`lemma_frame_out_empty_right);
+// // 		split (); smt ();
+// //                 ignore (forall_intros ()); ignore (implies_intro ());
 
-//                 split ();
+// //                 split ();
 
-//                 //case where Some tl_r
-// 		ignore (implies_intro ());
-// 		apply_lemma (`lemma_frame_out_empty_right);
-// 		split (); smt ();
+// //                 //case where Some tl_r
+// // 		ignore (implies_intro ());
+// // 		apply_lemma (`lemma_frame_out_empty_right);
+// // 		split (); smt ();
 
-//                 ignore (forall_intro ());  //tl_r binder, not needed
-// 		ignore (implies_intro ());
+// //                 ignore (forall_intro ());  //tl_r binder, not needed
+// // 		ignore (implies_intro ());
 
-//                 //important, this is where we are sending memory to the recursive call
-// 		apply_lemma (`lemma_rewrite_sep_comm);
-// 		apply_lemma (`lemma_frame_exact);
+// //                 //important, this is where we are sending memory to the recursive call
+// // 		apply_lemma (`lemma_rewrite_sep_comm);
+// // 		apply_lemma (`lemma_frame_exact);
 
-//                 split (); smt ();
-// 		//provide wp existentials for recursive call
-// 		witness (binder_to_term fl1_tail);
-// 		witness (binder_to_term fl2_binder);
-// 		witness (binder_to_term l1_tail_memory);
-// 		witness (binder_to_term m2_binder);
+// //                 split (); smt ();
+// // 		//provide wp existentials for recursive call
+// // 		witness (binder_to_term fl1_tail);
+// // 		witness (binder_to_term fl2_binder);
+// // 		witness (binder_to_term l1_tail_memory);
+// // 		witness (binder_to_term m2_binder);
 
-//                 //prove definedness/validity
-// 		split (); smt (); //boom! hail smt!
+// //                 //prove definedness/validity
+// // 		split (); smt (); //boom! hail smt!
 
-//                 //prove the postcondition part
-// 		ignore (forall_intros ());
-// 		let h = implies_intro () in __elim_and h;
-// 		let h = implies_intro () in __elim_and h;
-// 		ignore (implies_intros ());
-// 		split (); smt ();
+// //                 //prove the postcondition part
+// // 		ignore (forall_intros ());
+// // 		let h = implies_intro () in __elim_and h;
+// // 		let h = implies_intro () in __elim_and h;
+// // 		ignore (implies_intros ());
+// // 		split (); smt ();
 
-//                 //check this guy, both right and left seemed ok
-// 		apply_lemma (`lemma_frame_out_empty_left);
-// 		split (); smt ();
-// 		ignore (forall_intro ());
-// 		let h = implies_intro () in rewrite h;
-// 		split (); smt (); split (); smt ();
-// 		apply_lemma (`lemma_frame_out_empty_left);
-// 		split (); smt (); split (); smt (); split (); smt ();
-// 		apply_lemma (`lemma_frame_out_empty_left);
-// 		split (); smt (); split (); smt (); split (); smt (); split (); smt ();
-// 		apply_lemma (`lemma_frame_out_empty_left);
-// 		split (); smt (); split (); smt (); split (); smt ();
-// 		apply_lemma (`lemma_frame_out_empty_left);
-// 		smt ();
+// //                 //check this guy, both right and left seemed ok
+// // 		apply_lemma (`lemma_frame_out_empty_left);
+// // 		split (); smt ();
+// // 		ignore (forall_intro ());
+// // 		let h = implies_intro () in rewrite h;
+// // 		split (); smt (); split (); smt ();
+// // 		apply_lemma (`lemma_frame_out_empty_left);
+// // 		split (); smt (); split (); smt (); split (); smt ();
+// // 		apply_lemma (`lemma_frame_out_empty_left);
+// // 		split (); smt (); split (); smt (); split (); smt (); split (); smt ();
+// // 		apply_lemma (`lemma_frame_out_empty_left);
+// // 		split (); smt (); split (); smt (); split (); smt ();
+// // 		apply_lemma (`lemma_frame_out_empty_left);
+// // 		smt ();
 
-//                 //woot! done with the inductive case
+// //                 //woot! done with the inductive case
 
-//                 //now in the case when tl is None
-// 		ignore (implies_intro ());
-// 		apply_lemma (`lemma_inline_in_patterns_two);
-// 		split (); smt ();
-// 		split ();
-// 		ignore (implies_intro ());
-// 		apply_lemma (`lemma_frame_out_empty_right);
-// 		split (); smt ();
-// 		ignore (implies_intro ());
-// 		apply_lemma (`lemma_rw);
-// 		split (); smt (); split (); smt ();
-// 		apply_lemma (`lemma_frame_out_empty_left);
-// 		split (); smt ();
-// 		ignore (forall_intro ());
-// 		let h = implies_intro () in rewrite h;
-// 		split (); smt (); split (); smt ();
-// 		apply_lemma (`lemma_frame_out_empty_left);
-// 		split (); smt (); split (); smt (); split (); smt ();
-// 		apply_lemma (`lemma_frame_out_empty_left);
-// 		split (); smt (); split (); smt (); split (); smt ();
-// 		apply_lemma (`lemma_frame_out_empty_left);
-// 		split (); smt (); split (); smt (); split (); smt (); split (); smt ();
-// 		apply_lemma (`lemma_frame_out_empty_left);
-// 		split (); smt (); split (); smt (); split (); smt ();
-// 		apply_lemma (`lemma_frame_out_empty_left);
-// 		smt ();
-// 		smt ();
-// 		smt ();
-//                 dump "A")
+// //                 //now in the case when tl is None
+// // 		ignore (implies_intro ());
+// // 		apply_lemma (`lemma_inline_in_patterns_two);
+// // 		split (); smt ();
+// // 		split ();
+// // 		ignore (implies_intro ());
+// // 		apply_lemma (`lemma_frame_out_empty_right);
+// // 		split (); smt ();
+// // 		ignore (implies_intro ());
+// // 		apply_lemma (`lemma_rw);
+// // 		split (); smt (); split (); smt ();
+// // 		apply_lemma (`lemma_frame_out_empty_left);
+// // 		split (); smt ();
+// // 		ignore (forall_intro ());
+// // 		let h = implies_intro () in rewrite h;
+// // 		split (); smt (); split (); smt ();
+// // 		apply_lemma (`lemma_frame_out_empty_left);
+// // 		split (); smt (); split (); smt (); split (); smt ();
+// // 		apply_lemma (`lemma_frame_out_empty_left);
+// // 		split (); smt (); split (); smt (); split (); smt ();
+// // 		apply_lemma (`lemma_frame_out_empty_left);
+// // 		split (); smt (); split (); smt (); split (); smt (); split (); smt ();
+// // 		apply_lemma (`lemma_frame_out_empty_left);
+// // 		split (); smt (); split (); smt (); split (); smt ();
+// // 		apply_lemma (`lemma_frame_out_empty_left);
+// // 		smt ();
+// // 		smt ();
+// // 		smt ();
+// //                 dump "A")
+
